Continue Refinement Proof

Uppaal_Networks/AbsInt/AbsInt_Refine.thy
@@ -15,10 +15,34 @@ type_synonym 'a r_state_map = "(addr, 'a) mapping"
 fun r_lookup :: "('a::bot) r_state_map \<Rightarrow> addr \<Rightarrow> 'a" where
   "r_lookup m = Mapping.lookup_default \<bottom> m"
 
+instantiation mapping :: (type, "{preorder, bot}") preorder
+begin
+  definition less_eq_mapping :: "('a, 'b) mapping \<Rightarrow> ('a, 'b) mapping \<Rightarrow> bool" where
+  "C1 \<le> C2 \<longleftrightarrow> (\<forall>p. Mapping.lookup_default \<bottom> C1 p \<le> Mapping.lookup_default \<bottom> C2 p)"
+  
+  definition less_mapping :: "('a, 'b) mapping \<Rightarrow> ('a, 'b) mapping \<Rightarrow> bool" where
+  "less_mapping x y = (x \<le> y \<and> \<not> y \<le> x)"
+  
+  instance proof (standard, goal_cases)
+    case 1 show ?case by(simp add: less_mapping_def)
+  next
+    case 2 thus ?case by(auto simp: less_eq_mapping_def)
+  next
+    case 3 thus ?case using less_eq_mapping_def order_trans by fastforce
+  qed
+end
+
 definition RSM :: "('a::bot) r_state_map \<Rightarrow> 'a state_map" where
   "RSM m = SM (r_lookup m)"
 
 declare RSM_def[simp]
+
+lemma RSM_mono: "a \<le> b \<Longrightarrow> RSM a \<le> RSM b"
+proof -
+  assume "a \<le> b"
+  hence "lookup (RSM a) pc \<le> lookup (RSM b) pc" for pc by (simp add: less_eq_mapping_def)
+  thus ?thesis using less_eq_state_map_def by blast
+qed
 
 code_datatype RSM
 
@@ -29,8 +53,15 @@ lemma[code]: "\<bottom> = RSM r_empty_map"
 
 lemma[code]: "lookup (RSM m) = r_lookup m" by simp
 
-fun merge_single :: "('a::sup) state_map \<Rightarrow> addr \<Rightarrow> 'a \<Rightarrow> 'a state_map" where
+fun merge_single :: "('a::semilattice_sup) state_map \<Rightarrow> addr \<Rightarrow> 'a \<Rightarrow> 'a state_map" where
   "merge_single (SM m) pc x = SM (\<lambda>npc. if npc = pc then x \<squnion> m npc else m npc)"
+
+lemma merge_single_grows: "m \<le> merge_single m pc x"
+proof -
+  obtain mm where sm: "m = SM mm" using state_map_single_constructor by blast
+  have "lookup (SM mm) p \<le> lookup (merge_single (SM mm) pc x) p" for p by simp
+  from this sm show ?thesis using less_eq_state_map_def by blast
+qed
 
 fun r_merge_single :: "('a::{semilattice_sup, bot}) r_state_map \<Rightarrow> addr \<Rightarrow> 'a \<Rightarrow> 'a r_state_map" where
   "r_merge_single tree pc x = Mapping.update pc (x \<squnion> (r_lookup tree pc)) tree"
@@ -53,7 +84,7 @@ proof -
   from r l show ?thesis by simp
 qed
 
-lemma[code]: "merge_single (RSM m) pc x = RSM (r_merge_single m pc x)"
+lemma r_merge_single[code]: "merge_single (RSM m) pc x = RSM (r_merge_single m pc x)"
 proof(rule lookup_eq)
   obtain mm where func: "RSM m = SM mm" using state_map_single_constructor by blast
   have "(if k = pc then x \<squnion> mm k else mm k) = lookup (RSM (r_merge_single m pc x)) k" for k
@@ -64,10 +95,13 @@ proof(rule lookup_eq)
   thus "lookup (merge_single (RSM m) pc x) k = lookup (RSM (r_merge_single m pc x)) k" for k using func by auto
 qed
 
+lemma r_merge_single_grows: "m \<le> r_merge_single m pc x"
+  by (simp add: less_eq_mapping_def lookup_default_update')
+
 fun r_domain :: "('b::bot) r_state_map \<Rightarrow> addr set" where
   "r_domain tree = Set.filter (\<lambda>pc. r_lookup tree pc \<noteq> \<bottom>) (Mapping.keys tree)"
 
-lemma[code]: "domain (RSM m) = r_domain m"
+lemma r_domain[code]: "domain (RSM m) = r_domain m"
 proof (intro Set.equalityI Set.subsetI)
   fix x assume "x \<in> domain (RSM m)"
   hence lookup: "lookup (RSM m) x \<noteq> \<bottom>" by simp
@@ -77,15 +111,26 @@ proof (intro Set.equalityI Set.subsetI)
   from keys r_lookup show "x \<in> r_domain m" by auto
 qed auto
 
+lemma r_domain_finite: "finite (r_domain (Mapping m))" by (simp add: keys_Mapping)
+lemma domain_finite: "finite (domain (RSM (Mapping m)))" using r_domain r_domain_finite by metis
+
 lemma[code]: "astep_succs f op ipc st = {0, 1, 2, 3, 4, 5, 6, 7, 8, 9, 10}" (* TODO: this is completely wrong ofc *) sorry
 
-(* TODO: maybe first refine the algorithm, then the type,
-  but then the proof over the list won't work
-  can we still prove it? *)
+lemma fold_grow:
+  assumes "\<And>e acc. (acc::'a::preorder) \<le> f e acc"
+  shows "a \<le> fold f l a"
+proof(induction l arbitrary: a)
+  case (Cons x xs)
+  then show ?case using Cons.IH assms order_trans by fastforce
+qed simp
+
 fun r_step_map_from_with_op :: "('a::absstate) astep \<Rightarrow> instr \<Rightarrow> addr \<Rightarrow> 'a r_state_map \<Rightarrow> 'a r_state_map \<Rightarrow> 'a r_state_map" where
   "r_step_map_from_with_op f op ipc ctx acc = fold
     (\<lambda>pc acc. r_merge_single acc pc (f op ipc (r_lookup ctx ipc) pc))
     (sorted_list_of_set (astep_succs f op ipc (r_lookup ctx ipc))) acc"
+
+lemma r_step_map_from_with_op_grows: "acc \<le> r_step_map_from_with_op f op ipc ctx acc" using r_merge_single_grows fold_grow
+  by (metis (no_types, lifting) r_step_map_from_with_op.simps)
 
 fun r_step_map_from :: "('a::absstate) astep \<Rightarrow> program \<Rightarrow> 'a r_state_map \<Rightarrow> addr \<Rightarrow> 'a r_state_map \<Rightarrow> 'a r_state_map" where
   "r_step_map_from f prog ctx ipc acc =
@@ -93,29 +138,48 @@ fun r_step_map_from :: "('a::absstate) astep \<Rightarrow> program \<Rightarrow>
       Some op \<Rightarrow> r_step_map_from_with_op f op ipc ctx acc |
       None \<Rightarrow> acc)"
 
+lemma r_step_map_from_grows: "acc \<le> r_step_map_from f prog ctx ipc acc"
+  using r_step_map_from_with_op_grows by (cases "prog ipc"; simp)
+
 fun r_step_map :: "('a::absstate) astep \<Rightarrow> program \<Rightarrow> 'a r_state_map \<Rightarrow> 'a r_state_map" where
   "r_step_map f prog ctx = fold (r_step_map_from f prog ctx) (sorted_list_of_set (r_domain ctx)) \<bottom>"
 
 lemma sorted_list_of_set_split:
-  assumes "a \<in> s"
+  assumes "a \<in> s" "finite s"
   shows "\<exists>pre post. pre @ a # post = sorted_list_of_set s"
-  using assms(1) set_sorted_list_of_set split_list_first sorry
+  using assms set_sorted_list_of_set split_list_first by fastforce
 
-lemma[code]: "step_map (f::('a::absstate) astep) prog (RSM ctx) = RSM (r_step_map f prog ctx)"
+lemma fold_split:
+  "fold f (pre @ x # post) = fold f post \<circ> f x \<circ> fold f pre"
+  by simp
+
+lemma[code]: "step_map (f::('a::absstate) astep) prog (RSM (Mapping tree)) = RSM (r_step_map f prog (Mapping tree))"
 proof(rule lookup_eq)
-  have "\<Squnion>{ost. \<exists>ipc op. prog ipc = Some op \<and> r_lookup ctx ipc \<noteq> \<bottom> \<and> f op ipc (r_lookup ctx ipc) pc = ost} = r_lookup (r_step_map f prog ctx) pc" for pc
+  let ?ctx = "Mapping tree"
+  let ?smf = "r_step_map_from f prog ?ctx"
+  have "\<Squnion>{ost. \<exists>ipc op. prog ipc = Some op \<and> r_lookup ?ctx ipc \<noteq> \<bottom> \<and> f op ipc (r_lookup ?ctx ipc) pc = ost} = r_lookup (r_step_map f prog ?ctx) pc" for pc
   proof(rule Sup_eqI, goal_cases)
     case (1 ost)
-    then obtain ipc op where step: "prog ipc = Some op" "r_lookup ctx ipc \<noteq> \<bottom>" "f op ipc (r_lookup ctx ipc) pc = ost" by blast
-    obtain m where "SM m = RSM ctx" using state_map_single_constructor by metis
-    from this step have "ipc \<in> domain (RSM ctx)" by auto
-    then obtain pre post where "pre @ ipc # post = sorted_list_of_set (domain (RSM ctx))" sorry
-    then show ?case sorry
+    then obtain ipc op where step: "prog ipc = Some op" "r_lookup ?ctx ipc \<noteq> \<bottom>" "f op ipc (r_lookup ?ctx ipc) pc = ost" by blast
+    obtain m where "SM m = RSM ?ctx" using state_map_single_constructor by metis
+    from this step have "ipc \<in> domain (RSM ?ctx)" by auto
+    then obtain pre post where "pre @ ipc # post = sorted_list_of_set (domain (RSM ?ctx))" using sorted_list_of_set_split domain_finite by metis
+    hence "r_step_map f prog ?ctx = (fold ?smf post \<circ> ?smf ipc \<circ> fold ?smf pre) \<bottom>" using fold_split by (metis r_domain r_step_map.simps)
+    hence split: "r_step_map f prog ?ctx = fold ?smf post (?smf ipc (fold ?smf pre \<bottom>))" by simp
+    hence post:"?smf ipc (fold ?smf pre \<bottom>) \<le> r_step_map f prog ?ctx" by (metis fold_grow r_step_map_from_grows)
+    let ?prefold = "fold ?smf pre \<bottom>"
+    have "ost \<le> r_lookup (?smf ipc ?prefold) pc"
+    proof -
+      have rip: "?smf ipc ?prefold = r_step_map_from_with_op f op ipc ?ctx ?prefold" using step by simp
+      have "ost \<le> r_lookup (r_step_map_from_with_op f op ipc ?ctx ?prefold) pc" sorry
+      thus ?thesis using step rip by simp
+    qed
+    from post this show ?case using less_eq_mapping_def order_trans by fastforce
   next
     case (2 y)
     then show ?case sorry
   qed
-  thus "lookup (step_map f prog (RSM ctx)) pc = lookup (RSM (r_step_map f prog ctx)) pc" for pc by simp
+  thus "lookup (step_map f prog (RSM ?ctx)) pc = lookup (RSM (r_step_map f prog ?ctx)) pc" for pc by simp
 qed
 
 fun r_advance :: "('a::absstate) astep \<Rightarrow> program \<Rightarrow> 'a r_state_map \<Rightarrow> 'a r_state_map" where
